WIP: Imp to ModL.t

imp/Imp.v
@@ -198,7 +198,7 @@ End Denote.
 Section Interp.
 
   Context `{Σ: GRA.t}.
-  Definition effs := GlobEnv +' ImpState +' Es.
+  Definition effs := GlobEnv +' ImpState +' EventsL.Es.
 
   Definition handle_GlobEnv {eff} `{eventE -< eff} (ge: SkEnv.t) : GlobEnv ~> (itree eff) :=
     fun _ e =>
@@ -246,7 +246,7 @@ Section Interp.
     end
   .
 
-  Definition eval_imp (ge: SkEnv.t) (f: function) (args: list val) : itree Es val :=
+  Definition eval_imp (ge: SkEnv.t) (f: function) (args: list val) : itree EventsL.Es val :=
     match (init_args f.(fn_params) args []) with
     | Some iargs =>
       '(_, retv) <- (interp_imp ge (iargs++(init_lenv f.(fn_vars))) (denote_stmt f.(fn_body)));; Ret retv
@@ -271,6 +271,7 @@ Definition progFuns := list (gname * function).
 
 (** Imp program *)
 Record programL : Type := mk_programL {
+  nameL : list mname;
   ext_varsL : extVars;
   ext_funsL : extFuns;
   prog_varsL : progVars;
@@ -280,6 +281,7 @@ Record programL : Type := mk_programL {
 }.
 
 Record program : Type := mk_program {
+  name : mname;
   ext_vars : extVars;
   ext_funs : extFuns;
   prog_vars : progVars;
@@ -298,7 +300,7 @@ Record program : Type := mk_program {
 
 Definition lift (p : program) : programL :=
   mk_programL
-    p.(ext_vars) p.(ext_funs) p.(prog_vars) p.(prog_funs) p.(public) p.(defs).
+    [p.(name)] p.(ext_vars) p.(ext_funs) p.(prog_vars) p.(prog_funs) p.(public) p.(defs).
 
 Coercion lift : program >-> programL.
 (* Global Opaque imp_lift. *)
@@ -308,23 +310,21 @@ Module ImpMod.
 Section MODSEM.
 
   Context `{GRA: GRA.t}.
-  Variable mn: mname.
   Variable m: programL.
 
   Set Typeclasses Depth 5.
   (* Instance Initial_void1 : @Initial (Type -> Type) IFun void1 := @elim_void1. (*** TODO: move to ITreelib ***) *)
 
-  Definition modsem (ge: SkEnv.t) : ModSem.t := {|
-    ModSem.fnsems :=
+  Definition modsem (ge: SkEnv.t) : ModSemL.t := {|
+    ModSemL.fnsems :=
       List.map (fun '(fn, f) => (fn, cfun (eval_imp ge f))) m.(prog_funsL);
-    ModSem.mn := mn;
-    ModSem.initial_mr := ε;
-    ModSem.initial_st := tt↑;
+    ModSemL.initial_mrs :=
+      List.map (fun name => (name, (ε, tt↑))) m.(nameL);
   |}.
 
-  Definition get_mod: Mod.t := {|
-    Mod.get_modsem := fun ge => (modsem ge);
-    Mod.sk := m.(defsL);
+  Definition get_mod : ModL.t := {|
+    ModL.get_modsem := fun ge => (modsem ge);
+    ModL.sk := m.(defsL);
   |}.
 
 End MODSEM.
