imp_compile/ImpMem2.v
@@ -35,6 +35,7 @@ Section Mem2.
   |}.
 
   Definition imp_mem2_prog : program := {|
+    name := "Mem2";
     ext_vars := [];
     ext_funs := [];
     prog_vars := [];
